\documentclass[12pt]{article}
\usepackage{amsmath}
\usepackage{amssymb}
\usepackage{mathtools}
\usepackage{fancyhdr}
\pagestyle{fancy}
\setlength{\headheight}{15pt}
\lhead{\bfseries Group: SHPZKN}
\rhead{\bfseries ML Homework 7}

\newcommand\iideq{\stackrel{\tiny{\mbox{i.i.d}}}{=}}
\newcommand{\myexp}[1]{E\left[#1\right]}
\newcommand{\fh}[1][x]{\hat{f}(#1)}
\newcommand{\fhsq}[1][x]{\left(\hat{f}(#1)\right)^2}
\newcommand{\kbd}[2]{D_{KL}(#1||#2)}
\newcommand{\mysum}{\sum_{i=1}^N}
\newcommand{\mymin}{\underset{R}{min}}

\begin{document}
\section{Problem 1}
\paragraph{a)}
\begin{equation}
\begin{split}
Bias(\hat{\mu}) 
&= E\left(\hat{\mu} - \mu\right)
= E\left(\frac{1}{N}\sum_{i=1}^NX_i-\mu\right) \\     
&= E\left(\frac{1}{N}\sum_{i=1}^NX_i\right) - E\left(\mu\right)
= \frac{1}{N}E\left(\sum_{i=1}^NX_i\right) - \mu \\
&= \frac{1}{N}\sum_{i=1}^{N}E\left(X_i\right) - \mu 
\iideq \frac{N}{N}\mu - \mu \\
&= 0
\end{split}
\end{equation}
Since the $X_i$s are identically distributed, they have the same,
true, mean $\mu$.
\begin{equation}
\begin{split}
Var(\hat{\mu})
&= Var(\frac{1}{N}\sum_{i=1}^NX_i)
= \frac{1}{N^2}Var\left(\sum_{i=1}^NX_i\right) \\
&\iideq \frac{1}{N^2}\sum_{i=1}^NVar(X_i)
= \frac{N}{N^2}\sigma^2 \\
&= \frac{\sigma^2}{N}
\end{split}
\end{equation}
Note that $Cov(X_i, X_j) = 0\; \forall j\neq i$ because of independence.

\begin{equation}
\begin{split}
MSE(\hat{\mu})
&= \left(Bias(\hat{\mu})\right)^2 + Var(\hat{\mu}) \\
&= 0^2 + \frac{\sigma^2}{N} \\
&= \frac{\sigma^2}{N}
\end{split}
\end{equation}


\paragraph{b)}
\begin{equation}
\begin{split}
Bias(0) &= E\left(0 - \mu\right) \\
        &= -\mu
\end{split}
\end{equation}

\begin{equation}
\begin{split}
Var(0) = 0
\end{split}
\end{equation}
Since it is a constant and therefore not random.

\begin{equation}
\begin{split}
MSE(0) &= {\left(Bias(0)\right)}^2 + Var(0) \\
       &= {\left(-\mu\right)}^2 + 0 \\
       &= \mu^2
\end{split}
\end{equation}

\section{Problem 2}
\paragraph{a)}
\begin{equation}
\begin{split}
Error\left[\fh\right]
&= \myexp{(\fh - f(x))^2}  \\
&= \myexp{\fhsq - 2\fh f(x) + (f(x))^2} \\
&= \myexp{(\hat{f}(x))^2} - 2f(x)\myexp{\fh} + \left(f(x)\right)^2\\
&= \myexp{\fhsq}-2\left(\myexp{\fhsq}\right)^2 + \left(\myexp{\fhsq}\right)^2\\
&\quad + \left(E[\fhsq]\right)^2- 2f(x)E\left[\fh\right] + \left(f(x)\right)^2\\
&=\myexp{\fhsq} - 2\myexp{\fh\myexp{\fh}} + \myexp{\myexp{\fh}}^2\\
&\quad + \left(\myexp{\fh} - \myexp{f(x)}\right)^2\\
&= \myexp{\fhsq - 2\fh\myexp{\fhsq} + \myexp{\fhsq}}\\
&\quad + \left(\underbrace{\myexp{\fh} - f(x)}_{Bias}\right)^2\\
&= \underbrace{\myexp{\left(\fh - \myexp{\fh}\right)^2}}_{Var} + Bias^2\\
&= Var + Bias^2
\end{split}
\end{equation}
\section{Problem 3}
\paragraph{a)}
\begin{equation}
\begin{split}
\mymin A
&\stackrel{!}{=} \mymin \myexp{\kbd{R}{\hat{P}}}\\
&= \mymin \myexp{\mysum R_i \log \left(\frac{R_i}{\hat{P_i}}\right)}\\
&= \mymin \mysum \left(R_i \log R_i - R_i \myexp{\log \hat{P_i}} \right)
\end{split}
\end{equation}

\begin{equation}
\begin{split}
\frac{\partial A}{\partial R_i}
&= \log R_i + R_i \cdot \frac{1}{R_i} - \myexp{\log \hat{P_i}}\\
&= \log R_i + 1 - \myexp{\log \hat{P_i}} \stackrel{!}{=} 0\\
&\Leftrightarrow \log R_i = \myexp{\log \hat{P_i}} - 1\\
&\Leftrightarrow R_i = \frac{exp(\myexp{\log \hat{P_i}})}{exp(1)}\\
&\Leftrightarrow R_i = \frac{exp(\myexp{\log \hat{P_i}})}
                            {exp(\sum_{j=1}^C \hat{P_j})}
\end{split}
\end{equation}

\paragraph{b)}
\begin{equation}
\begin{split}
Error\left(\hat{P}\right)
&= \myexp{\kbd{P}{\hat{P}}}\\
&= \myexp{\mysum P_i \log\left(\frac{P_i}{\hat{P_i}}\right)}\\
&= \myexp{\mysum P_i \log\left(\frac{P_iR_i}{\hat{P_i}R_i}\right)}\\
&= \myexp{\mysum P_i\left(\log P_i-\log R_i + \log \hat{P_i} - \log R_i\right)}\\
&= \myexp{\mysum P_i \log\left(\frac{P_i}{R_i}\right) +
   \mysum P_i \log\left(\frac{R_i}{\hat{P_i}}\right)}\\
&= \mysum P_i \log\left(\frac{P_i}{R_i}\right) +
   \myexp{\mysum P_i \log\left(\frac{R_i}{\hat{P_i}}\right)}\\
&= \kbd{P}{R} + \myexp{\kbd{R}{\hat{P}}}\\
&= Bias\left(\hat{P}\right) + Var\left(\hat{P}\right)
\end{split}
\end{equation}

\end{document} 